tasks/extraction/basic_info/print_data.py
@@ -1,0 +1,10 @@
+#!/usr/bin/env python3
+from sqlitedict import SqliteDict
+
+def prt(pos):
+    return f"{pos.line}:{pos.column}"
+
+with SqliteDict('/lustre/scratch/users/qiyuan.xu/MLML_data/positions.db') as db:
+    for key, (value, _) in db.items():
+        for (cmd, prf, statement_begin, statement_end, proof_begin, proof_end) in value:
+            print(f"{key}, statement: {prt(statement_begin)} - {prt(statement_end)}, proof: {prt(proof_begin)} - {prt(proof_end)}. {cmd}\n {prf}\n\n")
