tasks/extraction/pretrain/unicode.py
@@ -1,0 +1,21 @@
+#!/usr/bin/env python3
+from IsaREPL import Client
+import sys
+import json
+
+if len(sys.argv) != 2:
+    print(f"Usage: {sys.argv[0]} <target jsonl file>")
+    sys.exit(1)
+path = sys.argv[1]
+
+def unicode(data):
+    data['text'] = Client.pretty_unicode(data['text'])
+    return data
+
+with open(path, 'r') as f:
+    DATA = [unicode(json.loads(line)) for line in f]
+
+with open(path, 'w') as f:
+    for data in DATA:
+        f.write(json.dumps(data))
+        f.write('\n')
