tasks/extraction/theorem-relevance/choose_valid.py
@@ -1,0 +1,83 @@
+#! /usr/bin/env python3
+import sqlite3
+import threading
+import random
+# import argparse
+from data.isabelle import PISA_Data
+from sqlitedict import SqliteDict
+import json
+
+# parser = argparse.ArgumentParser(description='Deduplicate premise relevance data')
+# parser.add_argument('db_path', default='./data/premise_relevance.db',
+#                     help='Path to the premise relevance database')
+# args = parser.parse_args()
+
+DB_PATH = './data/premise_relevance.db'
+VALIDATE_DB_PATH = './tasks/extraction/theorem-relevance/premise_relevance.validate.db'
+VALIDATE_IDX = './tasks/extraction/theorem-relevance/premise_relevance.validate.keys'
+
+db_conn = sqlite3.connect(DB_PATH)
+db_cursor = db_conn.cursor()
+db_cursor.execute('SELECT COUNT(*) FROM "unnamed"')
+TOTAL = db_cursor.fetchone()[0]
+
+data_provider = PISA_Data()
+PISA = set(data_provider.goal_pos_of(i).to_s(with_column=False) for i in data_provider.all_cases())
+PISA_KEYS = set()
+
+db_cursor.execute('SELECT key FROM "unnamed"')
+KEYS = set()
+for i, row in enumerate(db_cursor):
+    if i % 1000 == 0:
+        print(f"Processed {i} keys {TOTAL}")
+    parts = row[0].split(':')
+    key = f"{parts[0]}:{parts[1]}"
+    if key in PISA:
+        PISA_KEYS.add(key)
+        continue
+    KEYS.add(row[0])
+db_cursor.close()
+
+print(f"Total keys: {len(KEYS)}")
+
+def encode_goal(goal):
+    premises, concl = goal
+    return '|||'.join([premise for premise in premises] + [concl])
+
+KEY_list = list(KEYS)
+CHOSEN_KEYS = {}
+CHOSING_LOCKER = threading.Lock()
+CHOSEN_NUM = 50000
+MEET_GOALS = set()
+PAIRS = 0
+with SqliteDict(DB_PATH) as db:
+    for key in PISA_KEYS:
+        for goal, _ in db[key]:
+            MEET_GOALS.add(encode_goal(goal))
+    while len(CHOSEN_KEYS) < CHOSEN_NUM:
+        key = random.choice(KEY_list)
+        if key in CHOSEN_KEYS:
+            continue
+        value = db[key]
+        if len(value) != 1:
+            continue
+        goal, (ctxt, prems, goal_acs) = value[0]
+        #if len(prems) <= 2:
+        #    continue
+        if encode_goal(goal) in MEET_GOALS:
+            continue
+        MEET_GOALS.add(encode_goal(goal))
+        CHOSEN_KEYS[key] = value[0]
+        PAIRS += len(prems)
+        #print(f"Chosen one, with {len(prems)} premises and {len(goal_acs)} AC equivs")
+
+with SqliteDict(VALIDATE_DB_PATH) as db:
+    for key, value in CHOSEN_KEYS.items():
+        db[key] = [value]
+
+with open(VALIDATE_IDX, 'w') as f:
+    for key in CHOSEN_KEYS.keys():
+        f.write(key)
+        f.write("\n")
+
+print(f"Chosen {len(CHOSEN_KEYS)} keys, {PAIRS} pairs, written to {VALIDATE_DB_PATH} and {VALIDATE_IDX}")
