tasks/extraction/theorem-relevance/count_num.py
@@ -1,0 +1,10 @@
+from sqlitedict import SqliteDict
+
+NUM = 0
+with SqliteDict('/lustre/scratch/users/qiyuan.xu/MLML_data/premise_relevance.db') as db:
+    for i, (_, value) in enumerate(db.items()):
+        if i % 1000 == 0:
+            print(f"Processed {i} keys {NUM}")
+        lens = [len(r) for _, (_, r, _) in value]
+        NUM += sum(lens)
+print(NUM)
