tasks/extraction/theorem-relevance/graph_analysis.py
@@ -1,0 +1,112 @@
+from sqlitedict import SqliteDict
+import numpy as np
+from IsaREPL import Client
+from collections import Counter
+import io
+from scipy.sparse import csr_matrix, save_npz, load_npz
+
+# THMS = {}
+#GRAPH = {}
+INDEX = {}
+THM_OCCUR = Counter()
+#GOAL_OCCUR = Counter()
+
+THM_REL = {}
+THM_CSR = {}
+
+def encode_csr(mat: csr_matrix):
+    bio = io.BytesIO()
+    save_npz(bio, mat, compressed=True)
+    return bio.getvalue()
+
+def decode_csr(blob: bytes):
+    bio = io.BytesIO(blob)
+    return load_npz(bio)
+
+def mk_csr(counter: Counter, N: int):
+    cols = np.fromiter([INDEX[thm] for thm in counter.keys()], dtype=np.int32)
+    data = np.fromiter(counter.values(), dtype=np.float32)
+    rows = np.zeros_like(cols, dtype=np.int32)
+    v = csr_matrix((data, (rows, cols)), shape=(1, N), dtype=np.float32)
+    return v
+
+# def encode_goal(goal):
+#     premises, concl = goal
+#     premises = [Client.pretty_unicode(premise) for premise in premises]
+#     concl = Client.pretty_unicode(concl)
+#     goal = "###PREMISES\n" + "\n\n\n".join(premises) + "\n\n\n###CONCLUSION\n" + concl
+#     if goal.count("###PREMISES") > 1 or goal.count("###CONCLUSION") > 1:
+#         print("Warning: Found multiple occurrences of ###PREMISES or ###CONCLUSION in goal")
+#         exit(1)
+#     return goal
+
+     #SqliteDict('/lustre/scratch/users/qiyuan.xu/MLML_data/thm2thm_rel.db') as t2t_db
+with SqliteDict('/lustre/scratch/users/qiyuan.xu/MLML_data/premise_relevance.db') as db,\
+     SqliteDict('/lustre/scratch/users/qiyuan.xu/MLML_data/premise_info.db') as thm_db,\
+     SqliteDict('/lustre/scratch/users/qiyuan.xu/MLML_data/thm2thm_rel.db') as t2t_db:
+    # def get_premise(premise):
+    #     if premise in THMS:
+    #         return THMS[premise]
+    #     else:
+    #         try:
+    #             data = thm_db[premise]
+    #         except KeyError:
+    #             print(f"Warning: {premise} not found in thm_db")
+    #             exit(1)
+    #         defctxt, equivs = data
+    #         msg = defctxt + "\n" + "\n".join(equivs)
+    #         THMS[premise] = (defctxt, equivs)
+    #         return (defctxt, equivs)
+
+    num = 0
+    for _, data in db.items():
+        key, (_, thms, _) = data
+        THM_OCCUR.update(thms)
+        for thm in thms:
+            if thm not in THM_REL:
+                THM_REL[thm] = Counter()
+            THM_REL[thm].update(thms)
+            if thm not in INDEX:
+                INDEX[thm] = len(INDEX)
+        num += 1
+        if num % 1000 == 0:
+            print(f"Calculating Occurrence: Processed {num} keys")
+    N = len(INDEX)
+    TOTAL_NUMBER = mk_csr(THM_OCCUR, N)
+    # t2t_db['$THM_OCCUR'] = encode_csr(TOTAL_NUMBER)
+    # t2t_db.commit()
+    num = 0
+    for thm1, counter in THM_REL.items():
+        csr = mk_csr(counter, N)
+        THM_CSR[thm1] = csr
+        # t2t_db[thm1] = encode_csr(csr)
+        # num += 1
+        # if num % 100 == 0:
+        #     print(f"Processed {num} theorems")
+        #     t2t_db.commit()
+    print(f"CSR is built")
+    
+    for _, data in db.items():
+        key, (_, thms, _) = data
+        x = csr_matrix((1, N), dtype=np.float32)
+        for thm in thms:
+            PMI = THM_CSR[thm] * N / TOTAL_NUMBER[thm] / TOTAL_NUMBER
+            np.log(PMI.data, out=PMI.data)
+            np.maximum(PMI.data, 0, out=PMI.data)
+            PMI.eliminate_zeros()
+            
+
+
+        # goal = encode_goal(key)
+        # GOAL_OCCUR[goal] += 1
+        # if goal not in GRAPH:
+        #     GRAPH[goal] = Counter()
+        # GRAPH[goal].update(thms)
+    #for goal, counter in GRAPH.items():
+
+
+        #goal = dctxt + "\n###PREMISES\n" + "\n\n\n".join(premises) + "\n\n\n###CONCLUSION\n" + concl
+        
+
+        
+        
