tasks/extraction/theorem-relevance/mk_unicode.py
@@ -1,0 +1,12 @@
+from sqlitedict import SqliteDict
+from IsaREPL import Client, REPLFail
+
+with SqliteDict('/lustre/scratch/users/qiyuan.xu/MLML_data/premise_relevance.db') as db_org,\
+    SqliteDict('/lustre/scratch/users/qiyuan.xu/MLML_data/premise_info.db') as thm_db_org,\
+    SqliteDict('/lustre/scratch/users/qiyuan.xu/MLML_data/premise_relevance.unicode.db') as db,\
+    SqliteDict('/lustre/scratch/users/qiyuan.xu/MLML_data/premise_info.unicode.db') as thm_db:
+    for key, value in db_org.items():
+        premises, concl = key
+        premises = [Client.pretty_unicode(premise) for premise in premises]
+        concl = Client.pretty_unicode(concl)
+        key2 = (premises, concl)
