tasks/extraction/theorem-relevance/Premise_Extraction.thy
@@ -2,6 +2,7 @@ theory Premise_Extraction
   imports Minilang_Translator.MS_Translator Isa_REPL.Isa_REPL
 begin
 
+(* declare [[ML_debugger, ML_print_depth = 1000, ML_exception_trace, ML_exception_debugger]] *)
 
 ML_file "ac_shuffle.ML"
 
@@ -10,8 +11,369 @@ setup \<open>Context.theory_map (
   #> Theorem_Extraction.remove_AC [@{const_name HOL.eq}]
 )\<close>
 
+ML_file "context_info.ML"
 ML_file "sledgehammer.ML"
 ML_file "extraction.ML"
+
+
+(*
+ML \<open>fun f () = (\<^try>\<open>Syntax.read_term \<^context> "asdqq s!" catch e => error "OK"\<close>)\<close>
+
+term \<open>Par_Exn\<close>
+
+term 12
+ML \<open>f ()\<close>
+*)
+
+(*
+
+locale L0 =
+  fixes N :: \<open>'a :: times\<close>
+  assumes AX0: "N * N = N"
+
+locale L1 = L0 +
+  fixes P :: \<open>'a :: plus\<close> ("AA")
+    assumes A: "P = P"
+
+locale L2 = L1 0 1 +
+  fixes Q :: bool
+  assumes B: "Q"
+begin
+thm AX0
+
+definition "kkk = Q"
+
+thm L2_def
+thm L1_def
+thm L1_axioms_def
+
+end
+
+ML \<open>
+let val ctxt0 = Proof_Context.init_global \<^theory>
+    val ctxt = Target_Context.context_begin_named_cmd [] ("Premise_Extraction.L2", Position.none) \<^theory>
+ in Assumption.local_prems_of ctxt ctxt0
+  |> map (Simplifier.rewrite_rule ctxt @{thms L2_def L2_axioms_def } )
+    (* Variable.constraints_of ctxt *)
+end
+\<close>
+
+
+ML \<open>
+let val ctxt = Proof_Context.init_global \<^theory>
+    
+    val ctxt'= Locale.activate_declarations ("Premise_Extraction.L2", Morphism.identity) ctxt
+ in Assumption.local_assms_of ctxt' ctxt
+end
+\<close>
+
+
+
+fun fact where
+  "fact (0::nat) = 1" |
+  "fact (Suc N) = N * fact N"
+
+thm fact.simps 
+
+ML \<open>Thy_Info.get_names () |> List.app writeln\<close>
+
+
+
+term store
+ML \<open>Record.the_info \<^theory> "A_Aodv.state" |> #args\<close>
+thm state.simps
+thm store_def
+thm \<Gamma>\<^sub>A\<^sub>O\<^sub>D\<^sub>V_skeleton_simps(1)
+term PAodv
+ML \<open>Record.the_info \<^theory> \<close>
+
+thm non_trivial_neg
+
+thm non_trivial_neg
+  
+typ \<open>'a :: monoid_add\<close>
+ML \<open>Locale.axioms_of \<^theory> "DBM.class.time"\<close>
+typ \<open>'a :: DBM.time\<close>
+thm DBM.class.time_def
+thm class.time_axioms_def
+ML \<open>Locale.specification_of   \<^theory> "DBM.time"\<close>
+ 
+  
+ML \<open>      
+let val buf = Context_Info.mk_buffer ()
+    val info = Context_Info.defctxt_of \<^context> (Thm.prop_of @{thm non_trivial_neg})
+ in List.app (Context_Info.put_defctxt \<^context> buf) info
+  ; Context_Info.content_of buf |> tracing
+end \<close>
+
+term less_eq
+term\<open>\<infinity>\<close>
+thm dbm_lt.simps
+thm dbm_lt.intros
+ 
+ML \<open> 
+let val buf = Context_Info.mk_buffer ()
+    val info = Context_Info.defctxt_of \<^context> (Thm.prop_of @{thm dbm_not_lt_impl(1)})
+ in List.app (Context_Info.put_defctxt \<^context> buf) info
+  ; Context_Info.content_of buf |> tracing
+end \<close>
+
+term CHOICE
+
+typ AWN.seqp
+typ state
+record 'a xx =
+  aaa :: 'a
+  bbb :: \<open>'a \<times> 'a\<close>
+record yy = \<open>nat xx\<close> + zzz :: int
+term zzz
+term "Premise_Extraction.yy_ext"
+
+datatype ('a,'b) test = is_Test: Test (tA1: nat) 'b | Test2 (tB1: \<open>'a \<times> 'b\<close>) | is_Test3: Test3
+
+
+ML \<open>Record.the_info \<^theory> "Premise_Extraction.xx" |> #args\<close>
+ML \<open>Record.the_info \<^theory> "Premise_Extraction.yy" |> #parent\<close>
+
+consts AAA :: \<open>nat \<Rightarrow> nat \<Rightarrow> nat\<close> ("_ CC _")
+    
+term LABEL   
+
+ML \<open> 
+let val buf = Context_Info.mk_buffer ()
+ in Context_Info.put_ADT \<^context> buf
+      (the (Ctr_Sugar.ctr_sugar_of \<^context> "Premise_Extraction.test"),
+       BNF_Def.bnf_of \<^context> "Premise_Extraction.test")
+  ; Context_Info.content_of buf |> tracing
+end \<close>
+
+
+ML \<open> 
+let val buf = Context_Info.mk_buffer ()
+ in Context_Info.put_record \<^context> buf "Premise_Extraction.xx"
+  ; Context_Info.content_of buf
+end \<close>
+
+term Nil
+
+ML \<open>
+BNF_Def.bnf_of \<^context> "Premise_Extraction.test" |> the
+|> BNF_Def.map_of_bnf
+\<close>
+
+term aaa
+term rreqs
+
+
+term plus
+
+class semigroup_add = plus +
+  assumes add_assoc: "(a + b) + c = a + (b + c)"
+begin
+
+sublocale add: semigroup plus
+  by standard (fact add_assoc)
+
+declare add.assoc [algebra_simps, algebra_split_simps, field_simps, field_split_simps]
+
+end
+
+
+
+
+
+context L2 begin
+
+end
+
+term L2.kkk
+thm L2_def
+
+ML \<open>Locale.params_of \<^theory> "Premise_Extraction.L2"\<close>
+ML \<open>Locale.axioms_of \<^theory> "Premise_Extraction.L2"\<close>
+ML \<open>(oo)\<close>
+thm L2_def
+
+term plus
+ML \<open>Axclass.get_info \<^theory> "Groups.semigroup_add"\<close>
+ML \<open>Sign.super_classes \<^theory> "Groups.semigroup_add"\<close>
+ML \<open>Axclass.get_info \<^theory> "Groups.plus"\<close>
+
+ML \<open>
+fun show_const_syntax ctxt const_name =
+    let
+      val syn = Proof_Context.syntax_of ctxt
+      val prtabs = Syntax.prtabs syn
+      val tab = the_default Symtab.empty (AList.lookup (op =) prtabs "")
+      val entries = Symtab.lookup_list tab const_name
+    in
+      if null entries then
+        "No syntax for " ^ quote const_name
+      else
+        const_name ^ ": " ^ @{make_string} (entries)
+    end
+\<close>
+ML \<open>show_const_syntax \<^context> \<^const_syntax>\<open>LABEL\<close> |> tracing\<close>
+ML \<open>
+let val ctxt = Proof_Context.set_mode Proof_Context.mode_pattern \<^context>
+    val term = (Const (\<^const_name>\<open>LABEL\<close>, dummyT) $ Term.dummy $ Term.dummy)
+ in Syntax.string_of_term ctxt term
+ |> tracing
+end
+\<close>
+
+ML \<open>fun get_local_mixfixes (Local_Syntax.Syntax {mixfixes, ...}) = mixfixes\<close>
+ML \<open>Locale .params_of \<^theory> "Groups.semigroup_add"\<close>
+ML \<open>Locale.axioms_of \<^theory> "Groups.plus"\<close>
+ML \<open>Locale.pretty_locale \<^theory> false "Groups.monoid_add"\<close>
+ML \<open>Locale.pretty_locale \<^theory> false "Premise_Extraction.L2"\<close>
+thm class.monoid_add_def
+
+ML \<open>Locale.hyp_spec_of \<^theory> "Premise_Extraction.L1"\<close>
+ML \<open>
+let val dep = Locale.dest_dependencies [] \<^theory>
+    val m = filter (fn {target,...} => target = "Premise_Extraction.L2") dep
+  |> hd
+  |> #morphism
+    val m2 = filter (fn {target,...} => target = "Premise_Extraction.L1") dep
+              |> hd |> #morphism
+    val eles = Locale.hyp_spec_of \<^theory> "Premise_Extraction.L1"
+            |> map (Element.transform_ctxt m)
+    val mm = Morphism.compose m m2
+ in (* Locale.params_of \<^theory> "Premise_Extraction.L0"
+  |> map (Free o #1)
+  |> map (Morphism.term mm) *)
+  filter (fn {target,...} => target = "Premise_Extraction.L0")  dep
+(*Locale.hyp_spec_of \<^theory> "Premise_Extraction.L0"
+            |> map (Element.transform_ctxt mm)*)
+end
+\<close>
+
+ML \<open>Locale.axioms_of \<^theory> "Premise_Extraction.L2"
+      |> map (Simplifier.rewrite_rule \<^context> (Locale.get_unfolds \<^context>))\<close>
+thm L2_def
+thm L1_def
+ML \<open>Locale.get_unfolds \<^context>\<close>
+ML \<open>Locale.hyp_spec_of \<^theory> "Groups.monoid_add"\<close>
+ML \<open>Locale.params_of \<^theory> "Premise_Extraction.L2"\<close>
+ML \<open>Locale.params_of \<^theory> "Groups.semigroup_add"\<close>
+ML \<open>Locale.specification_of \<^theory> "Groups.plus"\<close>
+ML \<open>Name_Space.markup_table\<close>
+ML \<open>
+ local
+  val code =
+    "let \n\
+    \  fun symb_to_string (Printer.Arg p) = \"_[\" ^ Int.toString p ^ \"]\"\n\
+    \    | symb_to_string (Printer.TypArg p) = \"T[\" ^ Int.toString p ^ \"]\"\n\
+    \    | symb_to_string (Printer.String (_, s)) = quote s\n\
+    \    | symb_to_string (Printer.Break n) = \"break(\" ^ Int.toString n ^ \")\"\n\
+    \    | symb_to_string (Printer.Block (_, symbs)) = \n\
+    \        \"{\" ^ String.concatWith \" \" (map symb_to_string symbs) ^ \"}\"\n\
+    \in symb_to_string end"
+in
+  (* 尝试动态编译 *)
+  val symb_to_string_compiled =
+    ML_Context.eval_source (ML_Compiler.verbose false ML_Compiler.flags)
+      (Input.source false code (Position.none, Position.none))
+      
+end;
+
+\<close>
+
+ML \<open>
+fun get_mixfixes (Local_Syntax.Syntax {mixfixes, ...}) = mixfixes
+\<close>
+
+ML \<open>
+Locale.dest_dependencies [] \<^theory>
+  |> map (fn {source, target, ...} => (source, target))
+\<close>
+
+ML \<open>
+Named_Target.init
+\<close>
+
+ML \<open>
+
+fun activate_all name thy activ_elem (marked, input) =
+  let
+    val {parameters = (_, params), spec = (asm, defs), ...} = the_locale thy name;
+    val input' = input |>
+      (not (null params) ?
+        activ_elem (Element.Fixes (map (fn ((x, T), mx) => (Binding.name x, SOME T, mx)) params))) |>
+      (* FIXME type parameters *)
+      (case asm of SOME A => activ_elem (Assumes [(Binding.empty_atts, [(A, [])])]) | _ => I) |>
+      (not (null defs) ?
+        activ_elem (Element.Defines (map (fn def => (Binding.empty_atts, (def, []))) defs)));
+    val activate = activate_notes activ_elem (Context.Theory thy) NONE;
+  in
+    roundup thy activate Morphism.identity (name, Morphism.identity) (marked, input')
+  end
+
+fun pretty_locale thy show_facts name =
+  let
+    val locale_ctxt = Locale.init name thy;
+    fun cons_elem (elem as Element.Notes _) = show_facts ? cons elem
+      | cons_elem (elem as Element.Lazy_Notes _) = show_facts ? cons elem
+      | cons_elem elem = cons elem;
+    val elems =
+      Locale.activate_all name thy cons_elem (Symtab.empty, [])
+      |> snd |> rev
+      |> tap consolidate_notes
+      |> map force_notes;
+  in
+    Pretty.block (Pretty.keyword1 "locale" :: Pretty.brk 1 :: pretty_name locale_ctxt name ::
+      maps (fn elem => [Pretty.fbrk, Pretty.chunks (Element.pretty_ctxt locale_ctxt elem)]) elems)
+  end;
+\<close>
+
+term plus
+
+ML \<open>
+fun show_const_syntax_raw ctxt const_name =
+    let
+      val syn = Proof_Context.syntax_of ctxt
+      val prtabs = Syntax.prtabs syn
+      val tab = the_default Symtab.empty (AList.lookup (op =) prtabs "")
+      val entries = Symtab.lookup_list tab const_name
+    in
+       entries
+    end
+\<close>
+
+ML \<open>Syntax.print_syntax\<close>
+
+ML \<open>show_const_syntax_raw \<^context> \<^const_syntax>\<open>plus\<close> \<close>
+
+ML \<open>
+let val syn = Proof_Context.syntax_of @{context}
+    val prtabs = Syntax.prtabs syn
+    
+ in Printer.get_infix prtabs \<^const_syntax>\<open>Groups.plus_class.plus\<close>
+end \<close>
+
+ML \<open>Syntax.string_of_term \<^context> (Const(\<^const_name>\<open>Groups.plus_class.plus\<close>, dummyT)) |> tracing\<close>
+ML \<open>Name_Space.names_short\<close>
+ML \<open>Name_Space.extern\<close>
+ML \<open>Name_Space.extern \<^context> (Consts.space_of (Proof_Context.consts_of \<^context>)) "Groups.plus_class.plus"\<close>
+
+ML "\<^const_syntax>\<open>Groups.plus_class.plus\<close> |> String.explode"
+
+notation
+
+
+
+term Test
+term "is_Test"
+term "tA1"
+
+ML \<open>Ctr_Sugar.ctr_sugar_of \<^context> "Premise_Extraction.test" |> the |> #discs |> map (Thm.cterm_of \<^context>)\<close>
+ML \<open>Ctr_Sugar.ctr_sugar_of \<^context> "Premise_Extraction.test" |> the |> #selss\<close>
+ML \<open>Ctr_Sugar.ctr_sugar_of \<^context> "A_Aodv.state.state_ext" |> the |> #selss\<close>
+ML \<open>Ctr_Sugar.ctr_sugar_of \<^context> "Premise_Extraction.xx.xx_ext" |> the |> #ctrs\<close>
+ML \<open>String.substring ("0123456789", 3, 2)\<close>
+
+term "Inter"
 
 (*
 ML \<open>fun mapx F (L,x) = (map F L, F x)\<close>
@@ -47,6 +409,7 @@ fun print_term_ ctxt =
      in Syntax.string_of_term ctxt'
      #> REPL.trim_makrup
     end\<close>
+*)
 *)
 *)
 
