tasks/extraction/pretrain/Pretrain_Extraction.thy
@@ -1,0 +1,130 @@
+theory Pretrain_Extraction
+  imports Minilang_Translator.MS_Translator
+begin
+
+(* ML_file \<open>extraction.ML\<close> *)
+ML_file \<open>extraction2.ML\<close>
+
+(*
+ML \<open>val kwds = Thy_Header.get_keywords @{theory}\<close>
+ML \<open>
+Token.tokenize kwds {strict=false} (Input.source_explode (Input.string "show \" ?thesis \""))
+\<close>
+
+ML \<open>
+val contain_macro = exists (fn tok =>
+      let val s = Token.unparse tok
+       in String.isSubstring "?thesis" s orelse
+          String.isSubstring "?case" s
+      end )
+\<close>
+
+ML \<open>String.isSubstring "aa" "aaaa"\<close>
+
+ML \<open>val pos = Position.make {
+                  line=1, offset=1, end_offset=1,
+                  props= { label = "",
+                           file = "#REPL",
+                           id="" }
+                }\<close>
+ML \<open>fun end_pos_of shift pos =
+  Position.make {
+    line = the_default 0 (Position.line_of pos),
+    offset = the_default 1 (Position.end_offset_of pos) - 1 + shift,
+    end_offset = the_default 1 (Position.end_offset_of pos) + shift,
+    props= { label = the_default "" (Position.label_of pos),
+             file = the_default "" (Position.file_of pos),
+             id = the_default "" (Position.id_of pos) }
+  }
+
+fun last [] = error "no last"
+  | last [x] = x
+  | last (_ :: L) = last L
+
+fun parse_end_pos parser toks =
+  let val (ret, toks') = parser toks
+      val used = Token.pos_of (nth toks (length toks - length toks' - 1))
+   in ((ret, end_pos_of 0 used), toks')
+  end
+\<close>
+ML \<open>fun range scan = (Scan.ahead Parse.not_eof >> (Token.range_of o single)) -- scan >> Library.swap;\<close>
+
+lemma True
+proof auto
+qed
+  ML_val \<open> 
+Token.tokenize (Thy_Header.get_keywords @{theory}) {strict=false} (Symbol_Pos.explode (
+  "text \<open>sad\<close>", pos))
+|> Outer_Syntax.parse_span @{theory} (fn _ => error "aa")
+|> (fn tr =>
+  let val state = Toplevel.make_state (SOME @{theory})
+      val tr' = Toplevel.theory_to_proof (K (Toplevel.proof_of @{Isar.state})) Toplevel.empty
+   in Toplevel.command_exception false tr' state
+   |> Toplevel.command_exception false tr
+   |> Toplevel.proof_of
+   |> Proof.goal
+  end )
+\<close>
+
+ML \<open> 
+
+Token.tokenize (Thy_Header.get_keywords @{theory}) {strict=false} (Symbol_Pos.explode (
+  "show ?cases", pos))
+|> Outer_Syntax.parse_spans
+|> (fn Command_Span.Span (_, x)  :: _ => x)
+|> filter Token.is_proper
+|> tl
+|> map Token.kind_of
+\<close>
+
+
+lemma " x = (2::nat)"
+proof (cases x)
+  ML_val \<open>Toplevel.proof_of @{Isar.state} |> Proof.goal |> #goal\<close>
+  case 0
+  fix a :: int
+  { assume "x = 1" and "x = 2" hence "x + x = 2" by auto }
+  also
+  thm calculation
+  ML_val \<open>Proof_Context.get_thms (Toplevel.context_of @{Isar.state}) "calculation"\<close>
+  ML_val \<open>Toplevel.proof_of @{Isar.state} |> Proof.the_fact\<close>
+  then show ?thesis sorry
+next
+  
+  then show ?thesis sorry
+qed
+
+ML \<open>@{thm [[]]} |> Thm.prop_of\<close>
+
+(*
+Show all goals:
+  proof, next,
+  obtain, consider (*good or not?*)
+  unfolding,
+  tactics (turned off for elaborated proofs)
+
+  TODO!
+  interpretation, global_interpretation, subgoal
+
+Special:
+  assume - show full typed sorted expression
+Show facts:
+  using from with note a b c
+  using from with note a (*\<open>...\<close>*) b (*\<open>...\<close>*) c (*\<open>...\<close>*)
+
+Show this:
+  }
+  case
+  (*facts:
+    \<open>...\<close>
+    \<open>...\<close>*)
+Show calculation:
+  also finally
+  (*calculation: \<open>...\<close>*)
+Show goal (if contains ?thesis or ?)
+  show thus
+*)
+
+*)
+
+end
