tasks/extraction/theorem-relevance/Map.thy
@@ -1,0 +1,7 @@
+theory Map
+  imports Main
+begin
+
+consts xx :: int
+
+end
