init.sh
@@ -12,28 +12,27 @@ mkdir -p ./cache/downloads
 mkdir -p ./translation/results
 mkdir -p ./cache/translation/tmp
 
-# Check if md5sum file exists and verify database integrity
-if [ -f "./data/md5sum" ]; then
-    echo "Verifying database integrity..."
-    if md5sum --status -c ./data/md5sum; then
-        echo "Database integrity verified."
-    else
-        echo "Database files are out-of-date. Reinstalling..."
-        gunzip -f -k ./data/translation/declarations.db.gz
-        gunzip -f -k ./data/translation/results.db.gz
-        unzstd -f -k data/proof_context.db.zst
-        unzstd -f -k data/premise_selection/SH.pretty.db.zst
-        md5sum ./data/translation/declarations.db ./data/translation/results.db data/proof_context.db data/premise_selection/SH.pretty.db > ./data/md5sum
-    fi
-else
-    echo "Unpacking database files..."
-    gunzip -f -k ./data/translation/declarations.db.gz
-    gunzip -f -k ./data/translation/results.db.gz
-    unzstd -f -k data/proof_context.db.zst
-    unzstd -f -k data/premise_selection/SH.pretty.db.zst
-    md5sum ./data/translation/declarations.db ./data/translation/results.db > ./data/md5sum
-fi
-
+# # Check if md5sum file exists and verify database integrity
+# if [ -f "./data/md5sum" ]; then
+#     echo "Verifying database integrity..."
+#     if md5sum --status -c ./data/md5sum; then
+#         echo "Database integrity verified."
+#     else
+#         echo "Database files are out-of-date. Reinstalling..."
+#         gunzip -f -k ./data/translation/declarations.db.gz
+#         gunzip -f -k ./data/translation/results.db.gz
+#         unzstd -f -k data/proof_context.db.zst
+#         unzstd -f -k data/premise_selection/SH.pretty.db.zst
+#         md5sum ./data/translation/declarations.db ./data/translation/results.db data/proof_context.db data/premise_selection/SH.pretty.db > ./data/md5sum
+#     fi
+# else
+#     echo "Unpacking database files..."
+#     gunzip -f -k ./data/translation/declarations.db.gz
+#     gunzip -f -k ./data/translation/results.db.gz
+#     unzstd -f -k data/proof_context.db.zst
+#     unzstd -f -k data/premise_selection/SH.pretty.db.zst
+#     md5sum ./data/translation/declarations.db ./data/translation/results.db > ./data/md5sum
+# fi
 
 source ./envir.sh
 
@@ -55,7 +54,6 @@ if [[ "$reinstall_isabelle" == "y" ]]; then
     echo "Isabelle and AFP will be reinstalled."
 fi
 
-
 if md5sum --status -c ./contrib/Isabelle2024.md5sum; then
     echo "Isabelle2024 is up to date."
 else
@@ -70,16 +68,15 @@ fi
 read -p "Enter memory limit (in GB) for Isabelle (default: 50): " isabelle_memory
 isabelle_memory=${isabelle_memory:-50}
 
-# Validate that isabelle_memory is a positive integer and not less than 30
-if ! [[ "$isabelle_memory" =~ ^[0-9]+$ ]] || [ "$isabelle_memory" -lt 30 ]; then
-    echo "Error: Memory limit must be a positive integer greater or equal than 30GB"
-    exit 1
-fi
+# # Validate that isabelle_memory is a positive integer and not less than 30
+# if ! [[ "$isabelle_memory" =~ ^[0-9]+$ ]] || [ "$isabelle_memory" -lt 30 ]; then
+#     echo "Error: Memory limit must be a positive integer greater or equal than 30GB"
+#     exit 1
+# fi
 
 mkdir -p $(isabelle getenv -b ISABELLE_HOME_USER)/etc
 printf "ML_OPTIONS='--minheap 4G --maxheap ${isabelle_memory}G'\nML_MAX_HEAP=${isabelle_memory}" > $(isabelle getenv -b ISABELLE_HOME_USER)/etc/settings
 echo "Setting Isabelle memory limit to ${isabelle_memory}GB"
-
 
 #rm -f  $(isabelle getenv -b ISABELLE_HOME_USER)/etc/components 2>/dev/null
 isabelle components -u ./contrib/afp-2025-02-12/thys || exit 1
