tasks/extraction/theorem-relevance/Readme.md
@@ -1,0 +1,8 @@
+### Extraction
+
+./premise-extraction.py
+
+### Post Processing
+
+1. ./dedpu.py
+2. dump_data.py
